\newpage{}
\section{Appendix}

We assume in the following developments that the lookup function
$\ntherr : \forall \alpha. \alist{} \alpha \rightarrow \N \rightarrow \option{}
\alpha$ defined in the standard library is known by the reader.

\subsection{Equations on power series}

\label{interpR}

$$\begin{array}{lllcl}
\IR & & & : & \se \rightarrow \alist{} \mathtt{Rseq\_infty} \\
    & & &   & \rightarrow \option{} (\texttt{R} \rightarrow \texttt{R}) \\
\IR & (\mathtt{cnst}~ C & , \rho) & = & \return~ (\lambda \_.C)\\
\IR & (\mathtt{scal}~ C ~ E &, \rho) & = & \IR(E, \rho) \bind (\lambda f. \return (C * f))\\
\IR & (\mathtt{y} ~ i ~ k &, \rho) & = & \ntherr(\rho, i) \bind (\lambda u_n. \return (\Psum{}(u_n)^{(k)})) \\
\IR & (\mathtt{opp} ~E &, \rho) & = & \IR(E,\rho) \bind (\lambda f. \return (- f))\\
\IR & (\mathtt{plus} ~ E_1 ~ E_2 &, \rho) & = & \IR(E_1,\rho) \bind (\lambda f_1.\\
    & & &   & \IR(E_2,\rho) \bind (\lambda f_2. \return (f_1 + f_2)))\\
\end{array}$$


$$\left[\left| \_ \right|\right]_{\R} : \de \rightarrow \alist{}
\mathtt{Rseq\_infty} \rightarrow \Prop$$

\begin{center}
\begin{tabular}{c|c}
\begin{minipage}{0.45\textwidth}
$$\SemR{} = \bot$$
$$ \text{if } \left\lbrace
\begin{array}{ll}
& \IR(E_1, \rho) = \None\\
\text{or} & \IR(E_2, \rho) = \None
\end{array}\right.$$
\end{minipage}

& \begin{minipage}{0.45\textwidth}
$$\SemR{} = \forall x \in \R. e_1(x) = e_2(x)$$
$$\text{if } \left\lbrace
\begin{array}{ll}
& \IR(E_1, \rho) = \Some e_1\\
\text{and} & \IR(E_2, \rho) = \Some e_2
\end{array}\right.$$
\end{minipage}

\end{tabular}
\end{center}
\subsection{Equations on sequences over $\R$}

\label{interpN}
$$\begin{array}{lllcl}
\IN & & & : & \se \rightarrow \alist{} \Rseq \rightarrow \option{} \Rseq \\
\IN & (\mathtt{cnst}~ C & , \rho) & = & \return~ (\C{}(C))\\
\IN & (\mathtt{scal}~ C ~ E &, \rho) & = & \IN(E, \rho) \bind (\lambda u_n. \return (C * u_n))\\
\IN & (\mathtt{y} ~ i ~ k &, \rho) & = & \ntherr(\rho, i) \bind (\lambda u_n. \\
    & & &   & \return (\Dn{}(un,k)) \\
\IN & (\mathtt{opp} ~E &, \rho) & = & \IN(E,\rho) \bind (\lambda u_n. \return (- u_n))\\
\IN & (\mathtt{plus} ~ E_1 ~ E_2 &, \rho) & = & \IN(E_1,\rho) \bind (\lambda u_n.\\
    & & &   & \IN(E_2,\rho) \bind (\lambda v_n. \return (u_n + v_n)))\\
\end{array}$$

$$\left[\left| \_ \right|\right]_{\N} : \de \rightarrow \alist{}
\mathtt{Rseq\_infty} \rightarrow \Prop$$

\begin{center}
\begin{tabular}{c|c}
\begin{minipage}{0.45\textwidth}
$$\SemN{} = \bot$$
$$\text{if } \left\lbrace
\begin{array}{ll}
& \IN(E_1, \rho) = \None\\
\text{or} & \IN(E_2, \rho) = \None
\end{array}\right.$$
\end{minipage}

& \begin{minipage}{0.45\textwidth}
$$\SemN{} = \forall n \in \N. u_n(n) = v_n(n)$$
$$\text{if } \left\lbrace
\begin{array}{ll}
& \IN(E_1, \rho) = \Some u_n\\
\text{and} & \IN(E_2, \rho) = \Some v_n
\end{array}\right.$$
\end{minipage}

\end{tabular}
\end{center}
